\section{Coherent states}
What does a semiclassical state means?

Calculation work: $D(\alpha)=e^{-\frac{1}{2}|\alpha|^2}e^{\alpha a^{\dagger}}e^{\beta a}$. $D(\alpha)D^{\dagger}(\alpha)=1$. Take $\alpha$ and $\beta$ to be infintesimal, and expand the exponential in $D(\alpha)=e^{-\frac{1}{2}|\alpha|^2}e^{\alpha a^{\dagger}}e^{\beta a}$. Prove that when keeping only the linear terms,
$$
(1+\alpha\alpha^{\dagger}+\beta\alpha+\alpha^{*}a+\beta^{*}a^{\dagger})=1
$$
$$
\begin{aligned}
e^{-\frac{1}{2}|\alpha|^2}e^{\alpha a^{\dagger}}e^{\beta a}&\simeq 1.(1+\alpha a^{\dagger})(1+\beta a)\\
&\simeq 1+\alpha a^{\dagger}+\beta a 
\end{aligned}
$$
$$
(1+\alpha a^{\dagger}+\beta a )(1+\alpha^{*} a+\beta^{*} a^{\dagger} )\simeq 1+\alpha a^{\dagger}+\beta a+\alpha^{*} a+\beta^{*} a^{\dagger}
$$

Show that $D(\alpha e^{-i\omega t})\bket{0}=e^{-\frac{1}{2}|\alpha|^2}\exp[\alpha a^{\dagger}e^{-i\omega t}]\bket{0}$.
$$
\begin{aligned}
D(\alpha e^{-i\omega t})\bket{0}&=e^{-\frac{1}{2}|\alpha|^2}\exp[\alpha a^{\dagger}e^{-i\omega t}]\exp[-\alpha^{*}e^{i\omega t}a]\bket{0}\\
&=e^{-\frac{1}{2}|\alpha|^2}\exp[\alpha a^{\dagger}e^{-i\omega t}]\bket{0} (\text{ since }e^{\beta a}\bket{0}=\bket{0}, \beta =-\alpha^{*}e^{i\omega t})
\end{aligned}
$$


Show that $$
\brak{x}e^{\frac{i}{\hbar}(p_0X-x_0P)}\bket{0}=e^{\frac{i}{\hbar}p_0x}\psi_0(x-x_0,0)
$$
$$
\begin{aligned}
\brak{x}e^{\frac{i}{\hbar}(p_0X-x_0P)}&=\brak{x}e^{\frac{i}{\hbar}p_0X}e^{-\frac{i}{\hbar}x_0P}e^{-\frac{1}{2}[\frac{i}{\hbar}p_0X,-\frac{i}{\hbar}x_0P]}\\
&=\brak{x}e^{\frac{i}{\hbar}p_0X}e^{-\frac{i}{\hbar}x_0P}e^{-\frac{1}{2}x_0p_0(\frac{i}{\hbar})(-\frac{i}{\hbar})(i\hbar)}\\
&=\brak{x}e^{\frac{i}{\hbar}p_0X}e^{-\frac{i}{\hbar}x_0P}e^{-\frac{i}{\hbar}p_0\frac{x_0}{2}}\\
&=e^{\frac{i}{\hbar}p_0(x-\frac{x_0}{2})}\brak{x}e^{-\frac{i}{\hbar}x_0P}\\
&=e^{\frac{i}{\hbar}p_0(x-\frac{x_0}{2})}\brak{x}(e^{-\frac{i}{\hbar}(-x_0)P})^{\dagger}\\
&=e^{\frac{i}{\hbar}p_0(x-\frac{x_0}{2})}\brak{x-x_0}
\end{aligned}
$$